Computability/Constructions/Primitive.lean
@@ -8,7 +8,8 @@ import Computability.Basic
 /-!
 # Construction of basic primitive recursive functions
 
-This file defines basic primitive recursive codes for basic functions, such as if-else, or arithmetic functions.
+This file defines basic primitive recursive codes for basic functions, such as if-else, or
+arithmetic functions.
 
 ## Structure
 Each construction is roughly structured as follows.
@@ -24,10 +25,11 @@ Suppose we want to construct a primitive recursive function `f : ℕ → ℕ`.
     sometimes for large constructions, one needs to supply an argument to `apply_cp`
     to increase the search depth (e.g. `apply_cp 60`.)
 
-`@[simp] theorem c_f_evp {O : ℕ → ℕ} : evalp O c_f = f := by ...`
+`@[simp, evp_simps] theorem c_f_evp {O : ℕ → ℕ} : evalp O c_f = f := by ...`
   · theorem which asserts that the code `c_f` implements `f` upon evaluation with `evalp`.
 
-`@[simp] theorem c_f_ev {O : ℕ → ℕ} : eval O c_f = f := by rw [← evalp_eq_eval c_f_prim]; simp only [c_f_evp]`
+`@[simp] theorem c_f_ev {O : ℕ → ℕ} : eval O c_f = f := by`
+  `rw [← evalp_eq_eval c_f_prim]; simp only [c_f_evp]`
   · theorem which asserts that the code `c_f` implements `f` upon evaluation with `eval`.
     This follows "for free" once you have `c_f_evp `.
   
@@ -43,19 +45,27 @@ open Nat
 section comp₂
 namespace Oracle.Single.Code
 def comp₂ := fun c1 c2 c3 : Code => c1.comp (pair c2 c3)
-@[cp] theorem comp₂_prim {c1 c2 c3} (hc1 : code_prim c1) (hc2 : code_prim c2) (hc3 : code_prim c3) : code_prim (comp₂ c1 c2 c3) := by unfold comp₂; apply_cp
-@[simp] theorem comp₂_evp {O c1 c2 c3} : evalp O (comp₂ c1 c2 c3) = fun x => evalp O c1 ⟪evalp O c2 x, evalp O c3 x⟫ := by simp [comp₂,evalp];
-@[simp] theorem comp₂_ev {O c1 c2 c3} : eval O (comp₂ c1 c2 c3) = fun x => ⟪eval O c2 x, eval O c3 x⟫ >>= (eval O c1) := by simp [eval, comp₂, Seq.seq]
+@[cp] theorem comp₂_prim {c1 c2 c3} (hc1 : code_prim c1) (hc2 : code_prim c2) (hc3 : code_prim c3) :
+  code_prim (comp₂ c1 c2 c3) := by unfold comp₂; apply_cp
+@[simp, evp_simps] theorem comp₂_evp {O c1 c2 c3} :
+    evalp O (comp₂ c1 c2 c3) = fun x => evalp O c1 ⟪evalp O c2 x, evalp O c3 x⟫ := by
+  simp only [comp₂, evp_simps];
+@[simp] theorem comp₂_ev {O c1 c2 c3} :
+    eval O (comp₂ c1 c2 c3) = fun x => ⟪eval O c2 x, eval O c3 x⟫ >>= (eval O c1) := by
+  simp [eval, comp₂, Seq.seq]
 end Oracle.Single.Code
 end comp₂
 
 section comp₄
 namespace Oracle.Single.Code
 def comp₄ := fun c1 c2 c3 c4 c5 : Code => c1.comp₂ (pair c2 c3) (pair c4 c5)
-@[cp] theorem comp₄_prim {c1 c2 c3 c4 c5} (hc1 : code_prim c1) (hc2 : code_prim c2) (hc3 : code_prim c3) (hc4 : code_prim c4) (hc5 : code_prim c5) : code_prim (comp₄ c1 c2 c3 c4 c5) := by unfold comp₄; apply_cp
-@[simp] theorem comp₄_evp {O c1 c2 c3 c4 c5} : evalp O (comp₄ c1 c2 c3 c4 c5) = fun x ↦
+@[cp] theorem comp₄_prim {c1 c2 c3 c4 c5}
+  (hc1 : code_prim c1) (hc2 : code_prim c2)
+  (hc3 : code_prim c3) (hc4 : code_prim c4) (hc5 : code_prim c5) :
+  code_prim (comp₄ c1 c2 c3 c4 c5) := by unfold comp₄; apply_cp
+@[simp, evp_simps] theorem comp₄_evp {O c1 c2 c3 c4 c5} : evalp O (comp₄ c1 c2 c3 c4 c5) = fun x ↦
   evalp O c1 ⟪evalp O c2 x, evalp O c3 x, evalp O c4 x, evalp O c5 x⟫ := by
-  simp [comp₄,evalp, comp₂];
+  simp only [comp₄, evp_simps]
 @[simp] theorem comp₄_ev {O c1 c2 c3 c4 c5} : eval O (comp₄ c1 c2 c3 c4 c5) =
   fun x => ⟪eval O c2 x, eval O c3 x, eval O c4 x, eval O c5 x⟫
    >>= (eval O c1) := by
@@ -66,15 +76,16 @@ end comp₄
 section comp₃
 namespace Oracle.Single.Code
 def comp₃ := fun c1 c2 c3 c4 : Code => c1.comp₂ c2 (pair c3 c4)
-@[cp] theorem comp₃_prim {c1 c2 c3 c4} (hc1 : code_prim c1) (hc2 : code_prim c2) (hc3 : code_prim c3) (hc4 : code_prim c4) : code_prim (comp₃ c1 c2 c3 c4) := by unfold comp₃; apply_cp
-@[simp] theorem comp₃_evp {c1 c2 c3 c4} {O : ℕ → ℕ} : evalp O (comp₃ c1 c2 c3 c4) = fun x ↦
-  evalp O c1 ⟪evalp O c2 x, evalp O c3 x, evalp O c4 x⟫ := by
-  simp [comp₃,evalp]
+@[cp] theorem comp₃_prim {c1 c2 c3 c4}
+  (hc1 : code_prim c1) (hc2 : code_prim c2) (hc3 : code_prim c3) (hc4 : code_prim c4) :
+  code_prim (comp₃ c1 c2 c3 c4) := by unfold comp₃; apply_cp
+@[simp, evp_simps] theorem comp₃_evp {c1 c2 c3 c4} {O : ℕ → ℕ} :
+    evalp O (comp₃ c1 c2 c3 c4) = fun x ↦
+    evalp O c1 ⟪evalp O c2 x, evalp O c3 x, evalp O c4 x⟫ := by
+  simp only [comp₃, evp_simps]
 @[simp] theorem comp₃_ev {c1 c2 c3 c4} {O : ℕ → ℕ} : eval O (comp₃ c1 c2 c3 c4) = fun x ↦
-  ⟪eval O c2 x, eval O c3 x, eval O c4 x⟫ >>= (eval O c1)
- := by
+  ⟪eval O c2 x, eval O c3 x, eval O c4 x⟫ >>= (eval O c1) := by
     simp [comp₃, eval, comp₂, Seq.seq]
-
 end Oracle.Single.Code
 end comp₃
 
@@ -82,11 +93,12 @@ section id
 namespace Oracle.Single.Code
 def c_id := left.pair right
 @[cp] theorem c_id_prim : code_prim c_id := by unfold c_id; apply_cp
-@[simp] theorem c_id_evp {O : ℕ → ℕ} {n} : evalp O c_id n = n := by simp [c_id,evalp]
+@[simp, evp_simps] theorem c_id_evp {O : ℕ → ℕ} {n} : evalp O c_id n = n := by simp [c_id, evalp]
 theorem c_id_evp' {O : ℕ → ℕ} : evalp O c_id = id := by funext x; simp
 @[simp] theorem c_id_ev {O : ℕ → ℕ} {n} : eval O c_id n = n := by simp [c_id,eval,Seq.seq]
 end Oracle.Single.Code
-theorem Nat.PrimrecIn.id {O : ℕ → ℕ} : Nat.PrimrecIn O id := by rw [← c_id_evp']; exact code_prim_prop
+theorem Nat.PrimrecIn.id {O : ℕ → ℕ} : Nat.PrimrecIn O id := by
+  rw [← c_id_evp']; exact code_prim_prop
 end id
 
 section const
@@ -100,10 +112,10 @@ def c_const : ℕ → Code
   · unfold c_const
     expose_names
     exact code_prim.comp code_prim.succ h
-@[simp] theorem c_const_evp {O : ℕ → ℕ} : ∀ n m, evalp O (c_const n) m = n
+@[simp, evp_simps] theorem c_const_evp {O : ℕ → ℕ} : ∀ n m, evalp O (c_const n) m = n
 | 0, _ => rfl
 | n+1, m => by simp! [c_const_evp n m]
-@[simp] theorem c_const_ev {O : ℕ → ℕ}: ∀ n m, eval O (c_const n) m = n
+@[simp] theorem c_const_ev {O : ℕ → ℕ} : ∀ n m, eval O (c_const n) m = n
 | 0, _ => rfl
 | n+1, m => by simp! [c_const_ev n m]
 end Oracle.Single.Code
@@ -120,7 +132,7 @@ theorem _const_eq_c_const : c_const = Code.const := by
   unfold Code.const
   induction n
   · exact rfl
-  · simp
+  · simp only [comp.injEq, true_and]
     unfold c_const
     unfold Code.const
     expose_names
@@ -131,36 +143,44 @@ theorem _curry_eq_c_curry : c_curry = curry := by
   rw [_id_eq_c_id]
   rw [_const_eq_c_const]
 -- @[simp] theorem c_curry_prim : code_prim (c_curry c n) := by
-@[simp] theorem c_curry_evp {O : ℕ → ℕ} {c n x} : evalp O (c_curry c n) x = evalp O c ⟪n, x⟫ := by simp [c_curry,evalp]
-@[simp] theorem c_curry_ev {O : ℕ → ℕ} {c n x}: eval O (c_curry c n) x = eval O c ⟪n, x⟫ := by rw [_curry_eq_c_curry]; exact eval_curry c n x
+@[simp, evp_simps] theorem c_curry_evp {O : ℕ → ℕ} {c n x} :
+    evalp O (c_curry c n) x = evalp O c ⟪n, x⟫ := by simp [c_curry,evalp]
+@[simp] theorem c_curry_ev {O : ℕ → ℕ} {c n x} :
+    eval O (c_curry c n) x = eval O c ⟪n, x⟫ := by
+  rw [_curry_eq_c_curry]; exact eval_curry c n x
 end Oracle.Single.Code
 end curry
 
 section sgsg'
-/-- The signum function on naturals.  -/
+/-- The signum function on naturals. -/
 @[simp] def Nat.sg := fun x => if x=0 then 0 else 1
-/-- Maps zero to 1 and non-zero natural numbers to 0. This is the inverse of `Nat.sg` for boolean-like computations. -/
+/-- Maps zero to 1 and non-zero natural numbers to 0. This is the inverse of `Nat.sg` for
+boolean-like computations. -/
 @[simp] def Nat.sg' := fun x => if x=0 then 1 else 0
 namespace Oracle.Single.Code
 def c_sg := comp (prec zero (((c_const 1).comp left).comp left)) (pair zero c_id)
 @[cp] theorem c_sg_prim : code_prim c_sg := by unfold c_sg; apply_cp
-@[simp] theorem c_sg_evp {O : ℕ → ℕ} : evalp O c_sg = Nat.sg := by
-  simp [c_sg,evalp]
+@[simp, evp_simps] theorem c_sg_evp {O : ℕ → ℕ} : evalp O c_sg = Nat.sg := by
+  simp only [c_sg, evp_simps]
   funext n; induction n with
   | zero => exact rfl
   | succ n _ => simp
-@[simp] theorem c_sg_ev {O : ℕ → ℕ} : eval O c_sg = Nat.sg := by rw [← evalp_eq_eval c_sg_prim]; simp only [c_sg_evp]
+@[simp, evp_simps] theorem c_sg_ev {O : ℕ → ℕ} : eval O c_sg = Nat.sg := by
+  rw [← evalp_eq_eval c_sg_prim]; simp only [c_sg_evp]
 def c_sg' := comp (prec (c_const 1) (((zero).comp left).comp left)) (pair zero c_id)
 @[cp] theorem c_sg'_prim : code_prim c_sg' := by unfold c_sg'; apply_cp
-@[simp] theorem c_sg'_evp {O : ℕ → ℕ} : evalp O c_sg' = Nat.sg' := by
-  simp [c_sg',evalp]
+@[simp, evp_simps] theorem c_sg'_evp {O : ℕ → ℕ} : evalp O c_sg' = Nat.sg' := by
+  simp only [c_sg', evp_simps]
   funext n; induction n with
   | zero => exact rfl
   | succ n _ => simp
-@[simp] theorem c_sg'_ev {O : ℕ → ℕ} : eval O c_sg' = Nat.sg' := by rw [← evalp_eq_eval c_sg'_prim]; simp only [c_sg'_evp]
+@[simp, evp_simps] theorem c_sg'_ev {O : ℕ → ℕ} : eval O c_sg' = Nat.sg' := by
+  rw [← evalp_eq_eval c_sg'_prim]; simp only [c_sg'_evp]
 end Oracle.Single.Code
-theorem Nat.PrimrecIn.sg {O : ℕ → ℕ} : Nat.PrimrecIn O Nat.sg := by rw [←c_sg_evp]; exact code_prim_prop
-theorem Nat.PrimrecIn.sg' {O : ℕ → ℕ} : Nat.PrimrecIn O Nat.sg' := by rw [←c_sg'_evp]; exact code_prim_prop
+theorem Nat.PrimrecIn.sg {O : ℕ → ℕ} : Nat.PrimrecIn O Nat.sg := by
+  rw [← c_sg_evp]; exact code_prim_prop
+theorem Nat.PrimrecIn.sg' {O : ℕ → ℕ} : Nat.PrimrecIn O Nat.sg' := by
+  rw [← c_sg'_evp]; exact code_prim_prop
 @[simp] abbrev c_not := c_sg'
 end sgsg'
 
@@ -168,11 +188,14 @@ section n2b
 namespace Oracle.Single.Code
 def c_n2b := c_sg
 @[cp] theorem c_n2b_prim : code_prim c_n2b := by unfold c_n2b; apply_cp 10
-@[simp] theorem c_n2b_evp {O : ℕ → ℕ} : evalp O c_n2b = fun x => if n2b x = true then 1 else 0 := by
-  simp [c_n2b]
+@[simp, evp_simps] theorem c_n2b_evp {O : ℕ → ℕ} :
+    evalp O c_n2b = fun x => if n2b x = true then 1 else 0 := by
+  simp only [c_n2b, evp_simps]
   unfold Nat.sg; unfold n2b
   aesop
-@[simp] theorem c_n2b_ev {O : ℕ → ℕ} : eval O c_n2b = fun x => if n2b x = true then 1 else 0 := by rw [← evalp_eq_eval c_n2b_prim]; simp only [c_n2b_evp]; funext x; aesop
+@[simp, evp_simps] theorem c_n2b_ev {O : ℕ → ℕ} :
+    eval O c_n2b = fun x => if n2b x = true then 1 else 0 := by
+  rw [← evalp_eq_eval c_n2b_prim]; simp only [c_n2b_evp]; funext x; aesop
 end Oracle.Single.Code
 end n2b
 
@@ -180,61 +203,70 @@ section add
 namespace Oracle.Single.Code
 def c_add := (prec c_id ((succ.comp right).comp right))
 @[cp] theorem c_add_prim : code_prim c_add := by unfold c_add; apply_cp
-@[simp] theorem c_add_evp {O : ℕ → ℕ} : evalp O c_add = unpaired2 Nat.add := by
-  simp [c_add,evalp]
+@[simp, evp_simps] theorem c_add_evp {O : ℕ → ℕ} : evalp O c_add = unpaired2 Nat.add := by
+  simp only [c_add, evp_simps]
   funext n;
-  simp [unpaired2]
+  simp only [unpaired, unpair1_to_l, pair_r, succ_eq_add_one, unpair2_to_r, unpaired2, add_eq]
   induction n.r with
   | zero => exact rfl
   | succ n h => exact Nat.add_left_inj.mpr h
-@[simp] theorem c_add_ev {O : ℕ → ℕ} : eval O c_add = unpaired2 Nat.add := by rw [← evalp_eq_eval c_add_prim]; simp only [c_add_evp]
+@[simp, evp_simps] theorem c_add_ev {O : ℕ → ℕ} : eval O c_add = unpaired2 Nat.add := by
+  rw [← evalp_eq_eval c_add_prim]; simp only [c_add_evp]
 end Oracle.Single.Code
 end add
 section mul
 namespace Oracle.Single.Code
 def c_mul := prec zero (c_add.comp (pair left (right.comp right)))
 @[cp] theorem c_mul_prim : code_prim c_mul := by unfold c_mul; apply_cp
-@[simp] theorem c_mul_evp {O : ℕ → ℕ} : evalp O c_mul = unpaired2 Nat.mul := by
-  simp [c_mul,evalp]
+@[simp, evp_simps] theorem c_mul_evp {O : ℕ → ℕ} : evalp O c_mul = unpaired2 Nat.mul := by
+  simp only [c_mul, evp_simps]
   funext n;
-  simp [unpaired2]
+  simp only [unpaired, unpaired2, unpair1_to_l, pair_l, pair_r, add_eq, unpair2_to_r, mul_eq]
   induction n.r with
   | zero => exact rfl
   | succ n h =>
-    simp [*, mul_succ];
+    simp only [*, mul_succ];
     (expose_names; exact Nat.add_comm (unpair n_1).1 ((unpair n_1).1 * n))
-@[simp] theorem c_mul_ev {O : ℕ → ℕ} : eval O c_mul = unpaired2 Nat.mul := by rw [← evalp_eq_eval c_mul_prim]; simp only [c_mul_evp]
+@[simp, evp_simps] theorem c_mul_ev {O : ℕ → ℕ} : eval O c_mul = unpaired2 Nat.mul := by
+  rw [← evalp_eq_eval c_mul_prim]; simp only [c_mul_evp]
 end Oracle.Single.Code
 end mul
 section pow
 namespace Oracle.Single.Code
 def c_pow := prec (c_const 1) (c_mul.comp (pair (right.comp right) left))
 @[cp] theorem c_pow_prim : code_prim c_pow := by unfold c_pow; apply_cp
-@[simp] theorem c_pow_evp {O : ℕ → ℕ} : evalp O c_pow = unpaired2 Nat.pow := by
-  simp [c_pow,evalp]
+@[simp, evp_simps] theorem c_pow_evp {O : ℕ → ℕ} : evalp O c_pow = unpaired2 Nat.pow := by
+  simp only [c_pow, evp_simps]
   funext n;
-  simp [unpaired2]
-
+  simp only [unpaired, unpaired2, unpair1_to_l, pair_l, pair_r, unpair2_to_r, mul_eq]
   induction n.r with
   | zero => exact rfl
   | succ n h => simp [*, pow_succ];
-@[simp] theorem c_pow_ev {O : ℕ → ℕ} : eval O c_pow = unpaired2 Nat.pow := by rw [← evalp_eq_eval c_pow_prim]; simp only [c_pow_evp]
+@[simp, evp_simps] theorem c_pow_ev {O : ℕ → ℕ} : eval O c_pow = unpaired2 Nat.pow := by
+  rw [← evalp_eq_eval c_pow_prim]; simp only [c_pow_evp]
 end Oracle.Single.Code
 end pow
 
 section prec1
 namespace Oracle.Single.Code
 def c_prec1 (m) (cf : Code) := ((prec (c_const m) (cf.comp right)).comp (zero.pair c_id))
-@[cp] theorem c_prec1_prim {cf m} (hcf : code_prim cf) : code_prim (@c_prec1 m cf) := by unfold c_prec1; apply_cp
-@[simp] theorem c_prec1_evp {cf m} {O : ℕ → ℕ} : evalp O (c_prec1 m cf) = (fun n => n.rec m fun y IH => evalp O cf <| Nat.pair y IH) := by simp [c_prec1,evalp]
+@[cp] theorem c_prec1_prim {cf m} (hcf : code_prim cf) : code_prim (@c_prec1 m cf) := by
+  unfold c_prec1; apply_cp
+@[simp, evp_simps] theorem c_prec1_evp {cf m} {O : ℕ → ℕ} :
+    evalp O (c_prec1 m cf) = (fun n => n.rec m fun y IH => evalp O cf <| Nat.pair y IH) := by
+  simp [c_prec1,evalp]
 end Oracle.Single.Code
-theorem Nat.PrimrecIn.prec1 {cf m} {O : ℕ → ℕ} : Nat.PrimrecIn O (fun n => n.rec m fun y IH => evalp O cf <| Nat.pair y IH) := by rw [← c_prec1_evp]; exact code_prim_prop
+theorem Nat.PrimrecIn.prec1 {cf m} {O : ℕ → ℕ} :
+    Nat.PrimrecIn O (fun n => n.rec m fun y IH => evalp O cf <| Nat.pair y IH) := by
+  rw [← c_prec1_evp]; exact code_prim_prop
 end prec1
 section casesOn1
 namespace Oracle.Single.Code
 def c_casesOn1 (m) (cf : Code) := @c_prec1 m (cf.comp left)
-@[cp] theorem c_casesOn1_prim {cf m} (hcf : code_prim cf): code_prim (c_casesOn1 m cf) := by unfold c_casesOn1; apply_cp
-@[simp] theorem c_casesOn1_evp {cf m} {O : ℕ → ℕ} : evalp O (@c_casesOn1 m cf) = (Nat.casesOn · m (evalp O cf)) := by simp [c_casesOn1,evalp]
+@[cp] theorem c_casesOn1_prim {cf m} (hcf : code_prim cf) :
+  code_prim (c_casesOn1 m cf) := by unfold c_casesOn1; apply_cp
+@[simp, evp_simps] theorem c_casesOn1_evp {cf m} {O : ℕ → ℕ} :
+  evalp O (@c_casesOn1 m cf) = (Nat.casesOn · m (evalp O cf)) := by simp [c_casesOn1,evalp]
 end Oracle.Single.Code
 end casesOn1
 
@@ -242,37 +274,43 @@ section pred
 namespace Oracle.Single.Code
 def c_pred := (c_casesOn1 0 c_id)
 @[cp] theorem c_pred_prim : code_prim c_pred := by unfold c_pred; apply_cp
-@[simp] theorem c_pred_evp {O : ℕ → ℕ} : evalp O c_pred = Nat.pred := by
-  simp [c_pred]
+@[simp, evp_simps] theorem c_pred_evp {O : ℕ → ℕ} : evalp O c_pred = Nat.pred := by
+  simp only [c_pred]
   funext n;
   cases n <;> simp [*]
-@[simp] theorem c_pred_ev {O : ℕ → ℕ} : eval O c_pred = Nat.pred := by rw [← evalp_eq_eval c_pred_prim]; simp only [c_pred_evp]
+@[simp, evp_simps] theorem c_pred_ev {O : ℕ → ℕ} : eval O c_pred = Nat.pred := by
+  rw [← evalp_eq_eval c_pred_prim]; simp only [c_pred_evp]
 end Oracle.Single.Code
 end pred
 section sub
 namespace Oracle.Single.Code
 def c_sub := prec c_id ((c_pred.comp right).comp right)
 @[cp] theorem c_sub_prim : code_prim c_sub := by unfold c_sub; apply_cp
-@[simp] theorem c_sub_evp {O : ℕ → ℕ} : evalp O c_sub = unpaired2 Nat.sub := by
-  simp [c_sub,evalp]
+@[simp, evp_simps] theorem c_sub_evp {O : ℕ → ℕ} : evalp O c_sub = unpaired2 Nat.sub := by
+  simp only [c_sub, evp_simps]
   funext n;
-  simp [unpaired2]
+  simp? [unpaired2] says
+    simp only [unpaired, unpair1_to_l, pair_r, pred_eq_sub_one, unpair2_to_r, unpaired2, sub_eq]
   induction n.r with
   | zero => exact rfl
   | succ n h =>
     simp [*, Nat.sub_add_eq];
-@[simp] theorem c_sub_ev {O : ℕ → ℕ} : eval O c_sub = unpaired2 Nat.sub := by rw [← evalp_eq_eval c_sub_prim]; simp only [c_sub_evp]
+@[simp, evp_simps] theorem c_sub_ev {O : ℕ → ℕ} : eval O c_sub = unpaired2 Nat.sub := by
+  rw [← evalp_eq_eval c_sub_prim]; simp only [c_sub_evp]
 end Oracle.Single.Code
 end sub
 section dist
 namespace Oracle.Single.Code
 def c_dist := c_add.comp (pair c_sub (c_sub.comp (pair right left)))
 @[cp] theorem c_dist_prim : code_prim c_dist := by unfold c_dist; apply_cp
-@[simp] theorem c_dist_evp {O : ℕ → ℕ} : evalp O c_dist = unpaired2 Nat.dist := by simp [c_dist,evalp]; exact rfl
-@[simp] theorem c_dist_ev {O : ℕ → ℕ} : eval O c_dist = unpaired2 Nat.dist := by rw [← evalp_eq_eval c_dist_prim]; simp only [c_dist_evp]
+@[simp, evp_simps] theorem c_dist_evp {O : ℕ → ℕ} : evalp O c_dist = unpaired2 Nat.dist := by
+  simp only [c_dist, evp_simps]; simp only [unpaired2, sub_eq, pair_l, pair_r, add_eq]; exact rfl
+@[simp, evp_simps] theorem c_dist_ev {O : ℕ → ℕ} : eval O c_dist = unpaired2 Nat.dist := by
+  rw [← evalp_eq_eval c_dist_prim]; simp only [c_dist_evp]
 end Oracle.Single.Code
 end dist
-@[simp] theorem eq_zero_iff_dist_zero {a b : ℕ} : a.dist b = 0 ↔ a=b := ⟨fun x ↦ Nat.eq_of_dist_eq_zero x, fun x ↦ Nat.dist_eq_zero x⟩
+@[simp] theorem eq_zero_iff_dist_zero {a b : ℕ} : a.dist b = 0 ↔ a=b :=
+  ⟨fun x ↦ Nat.eq_of_dist_eq_zero x, fun x ↦ Nat.dist_eq_zero x⟩
 theorem sgdist_eq_ifeq {a b : ℕ} : (if a.dist b = 0 then 0 else 1) = (if a=b then 0 else 1) := by
   simp only [eq_zero_iff_dist_zero]
 
@@ -281,9 +319,13 @@ namespace Oracle.Single.Code
 /-- eval c_if_eq' (x,y) = [x=y] -/
 def c_if_eq' := c_sg.comp c_dist
 @[cp] theorem c_if_eq'_prim : code_prim c_if_eq' := by unfold c_if_eq'; apply_cp
-@[simp] theorem c_if_eq'_evp {O : ℕ → ℕ} : evalp O c_if_eq' = fun ab => if ab.l=ab.r then 0 else 1 := by simp [c_if_eq',evalp];
-@[simp] theorem c_if_eq'_ev {O : ℕ → ℕ} : eval O c_if_eq' = fun ab => if ab.l=ab.r then Part.some 0 else Part.some 1 := by
-  rw [← evalp_eq_eval c_if_eq'_prim]; simp only [c_if_eq'_evp]; funext xs; exact apply_ite Part.some (xs.l = xs.r) 0 1
+@[simp, evp_simps] theorem c_if_eq'_evp {O : ℕ → ℕ} :
+    evalp O c_if_eq' = fun ab => if ab.l=ab.r then 0 else 1 := by
+  simp [c_if_eq', evp_simps];
+@[simp] theorem c_if_eq'_ev {O : ℕ → ℕ} :
+    eval O c_if_eq' = fun ab => if ab.l=ab.r then Part.some 0 else Part.some 1 := by
+  rw [← evalp_eq_eval c_if_eq'_prim]; simp only [c_if_eq'_evp]; funext xs;
+  exact apply_ite Part.some (xs.l = xs.r) 0 1
 end Oracle.Single.Code
 end if_eq'
 
@@ -301,21 +343,25 @@ def c_if_eq_te :=
   have cp_eq : code_prim eq := by apply_cp;
   apply_cp
 
-@[simp] theorem c_if_eq_te_evp {O : ℕ → ℕ} {a b c d} : evalp O c_if_eq_te ⟪a,b,c,d⟫ = if a=b then c else d := by
-  simp [c_if_eq_te,evalp];
+@[simp, evp_simps] theorem c_if_eq_te_evp {O : ℕ → ℕ} {a b c d} :
+    evalp O c_if_eq_te ⟪a,b,c,d⟫ = if a=b then c else d := by
+  simp only [c_if_eq_te];
   cases Classical.em (a=b) with
   | inl h => simp [h]
   | inr h => simp [h]
-@[simp] theorem c_if_eq_te_ev {O : ℕ → ℕ} {a b c d} : eval O c_if_eq_te ⟪a,b,c,d⟫ = if a=b then c else d := by
+@[simp] theorem c_if_eq_te_ev {O : ℕ → ℕ} {a b c d} :
+    eval O c_if_eq_te ⟪a,b,c,d⟫ = if a=b then c else d := by
   rw [← evalp_eq_eval c_if_eq_te_prim];
   simp
-theorem c_if_eq_te_evp' {O : ℕ → ℕ} : evalp O c_if_eq_te = fun x => if x.l.l=x.l.r then x.r.l else x.r.r := by
-  simp [c_if_eq_te,evalp];
+theorem c_if_eq_te_evp' {O : ℕ → ℕ} :
+    evalp O c_if_eq_te = fun x => if x.l.l=x.l.r then x.r.l else x.r.r := by
+  simp only [c_if_eq_te, evp_simps];
   funext xs
   cases Classical.em (xs.l.l=xs.l.r) with
   | inl h => simp [h]
   | inr h => simp [h]
-theorem c_if_eq_te_ev' {O : ℕ → ℕ} : eval O c_if_eq_te = fun x => if x.l.l=x.l.r then x.r.l else x.r.r := by
+theorem c_if_eq_te_ev' {O : ℕ → ℕ} :
+    eval O c_if_eq_te = fun x => if x.l.l=x.l.r then x.r.l else x.r.r := by
   rw [← evalp_eq_eval c_if_eq_te_prim]; simp only [c_if_eq_te_evp']; funext xs;
   cases Classical.em (xs.l.l=xs.l.r) with
   | inl h => simp [h]
@@ -328,22 +374,22 @@ namespace Oracle.Single.Code
 /-- eval c_if_lt_te (x,y) = [x<y] -/
 def c_if_lt_te :=
   let lt := c_sg.comp <| c_sub.comp₂ (succ.comp <| left.comp left) (right.comp left);
-
   c_add.comp₂
   (c_mul.comp₂ lt (right.comp right))
   (c_mul.comp₂ (c_not.comp lt) (left.comp right))
 @[cp] theorem c_if_lt_te_prim : code_prim c_if_lt_te := by
   repeat (first|assumption|apply_rules using cp|simp|constructor)
-@[simp] theorem c_if_lt_te_evp {O : ℕ → ℕ} {a b c d} : evalp O c_if_lt_te ⟪a,b,c,d⟫ = if a<b then c else d := by
-  simp [c_if_lt_te,evalp];
-  -- funext xs
+@[simp, evp_simps] theorem c_if_lt_te_evp {O : ℕ → ℕ} {a b c d} :
+    evalp O c_if_lt_te ⟪a,b,c,d⟫ = if a<b then c else d := by
+  simp only [c_if_lt_te, evp_simps];
   cases Classical.em (a<b) with
   | inl h => simp [h, Nat.sub_eq_zero_of_le h]
   | inr h =>
     have h1: a+1-b>0 := by exact tsub_pos_iff_not_le.mpr h
     have h0: ¬(a+1-b=0) := by exact Nat.ne_zero_of_lt h1
     simp [h, h0]
-@[simp] theorem c_if_lt_te_ev {O : ℕ → ℕ} {a b c d} : eval O c_if_lt_te ⟪a,b,c,d⟫ = if a<b then c else d := by
+@[simp] theorem c_if_lt_te_ev {O : ℕ → ℕ} {a b c d} :
+    eval O c_if_lt_te ⟪a,b,c,d⟫ = if a<b then c else d := by
   rw [← evalp_eq_eval c_if_lt_te_prim]; simp
 end Oracle.Single.Code
 end if_lt_te
@@ -352,15 +398,17 @@ section if_le_te
 namespace Oracle.Single.Code
 -- we use the fact that `a<b+1 ↔ a ≤ b`.
 /-- eval c_if_le_te (x,y) = [x ≤ y] -/
-def c_if_le_te := c_if_lt_te.comp (pair (pair (left.comp left) (succ.comp <| right.comp left)) right)
+def c_if_le_te :=
+  c_if_lt_te.comp (pair (pair (left.comp left) (succ.comp <| right.comp left)) right)
 @[cp] theorem c_if_le_te_prim : code_prim c_if_le_te := by unfold c_if_le_te; apply_cp
-@[simp] theorem c_if_le_te_evp {O : ℕ → ℕ} {a b c d} : evalp O c_if_le_te ⟪a,b,c,d⟫ = if a ≤ b then c else d := by
-  simp [c_if_le_te,evalp];
-  -- funext xs
+@[simp, evp_simps] theorem c_if_le_te_evp {O : ℕ → ℕ} {a b c d} :
+    evalp O c_if_le_te ⟪a,b,c,d⟫ = if a ≤ b then c else d := by
+  simp only [c_if_le_te, evp_simps];
   cases Classical.em (a<b+1) with
   | inl h => simp [h, Nat.lt_add_one_iff.mp h]
   | inr h => simp [h, Nat.lt_add_one_iff.not.mp h]
-@[simp] theorem c_if_le_te_ev {O : ℕ → ℕ} {a b c d} : eval O c_if_le_te ⟪a,b,c,d⟫ = if a ≤ b then c else d := by
+@[simp] theorem c_if_le_te_ev {O : ℕ → ℕ} {a b c d} :
+    eval O c_if_le_te ⟪a,b,c,d⟫ = if a ≤ b then c else d := by
   rw [← evalp_eq_eval c_if_le_te_prim]; simp
 end Oracle.Single.Code
 end if_le_te
@@ -370,21 +418,22 @@ namespace Oracle.Single.Code
 /-- eval c_flip (x,y) = (y,x) -/
 def c_flip := pair right left
 @[cp] theorem c_flip_prim : code_prim c_flip := by unfold c_flip; apply_cp
-@[simp] theorem c_flip_evp {O : ℕ → ℕ} {a b} : evalp O c_flip ⟪a, b⟫ = ⟪b, a⟫ := by
-  simp [c_flip,evalp];
+@[simp, evp_simps] theorem c_flip_evp {O : ℕ → ℕ} {a b} : evalp O c_flip ⟪a, b⟫ = ⟪b, a⟫ := by
+  simp [c_flip, evp_simps];
 @[simp] theorem c_flip_ev {O : ℕ → ℕ} {a b} : eval O c_flip ⟪a, b⟫ = ⟪b, a⟫ := by
   rw [← evalp_eq_eval c_flip_prim]; simp
 end Oracle.Single.Code
 end flip
-
 
 section if_gt_te
 namespace Oracle.Single.Code
 /-- eval c_if_gt_te (x,y) = [x>y] -/
 def c_if_gt_te := c_if_lt_te.comp (pair (c_flip.comp left) right)
 @[cp] theorem c_if_gt_te_prim : code_prim c_if_gt_te := by unfold c_if_gt_te; apply_cp
-@[simp] theorem c_if_gt_te_evp {O : ℕ → ℕ} {a b c d} : evalp O c_if_gt_te ⟪a,b,c,d⟫ = if a>b then c else d := by simp [c_if_gt_te,evalp];
-@[simp] theorem c_if_gt_te_ev {O : ℕ → ℕ} {a b c d} : eval O c_if_gt_te ⟪a,b,c,d⟫ = if a>b then c else d := by
+@[simp, evp_simps] theorem c_if_gt_te_evp {O : ℕ → ℕ} {a b c d} :
+    evalp O c_if_gt_te ⟪a,b,c,d⟫ = if a>b then c else d := by simp [c_if_gt_te, evp_simps];
+@[simp] theorem c_if_gt_te_ev {O : ℕ → ℕ} {a b c d} :
+    eval O c_if_gt_te ⟪a,b,c,d⟫ = if a>b then c else d := by
   rw [← evalp_eq_eval c_if_gt_te_prim]; simp
 end Oracle.Single.Code
 end if_gt_te
@@ -393,25 +442,33 @@ namespace Oracle.Single.Code
 /-- eval c_if_ge_te (x,y) = [x>y] -/
 def c_if_ge_te := c_if_le_te.comp (pair (c_flip.comp left) right)
 @[cp] theorem c_if_ge_te_prim : code_prim c_if_ge_te := by unfold c_if_ge_te; apply_cp
-@[simp] theorem c_if_ge_te_evp {O : ℕ → ℕ} {a b c d} : evalp O c_if_ge_te ⟪a,b,c,d⟫ = if a≥b then c else d := by simp [c_if_ge_te,evalp];
-@[simp] theorem c_if_ge_te_ev {O : ℕ → ℕ} {a b c d} : eval O c_if_ge_te ⟪a,b,c,d⟫ = if a≥b then c else d := by
+@[simp, evp_simps] theorem c_if_ge_te_evp {O : ℕ → ℕ} {a b c d} :
+  evalp O c_if_ge_te ⟪a,b,c,d⟫ = if a≥b then c else d := by simp [c_if_ge_te, evp_simps];
+@[simp] theorem c_if_ge_te_ev {O : ℕ → ℕ} {a b c d} :
+    eval O c_if_ge_te ⟪a,b,c,d⟫ = if a≥b then c else d := by
   rw [← evalp_eq_eval c_if_ge_te_prim]; simp
 end Oracle.Single.Code
 end if_ge_te
 
 section ifz
 namespace Oracle.Single.Code
-def c_ifz := c_add.comp <| pair (c_mul.comp <| pair (c_sg'.comp left) (left.comp right)) (c_mul.comp <| pair (c_sg.comp left) (right.comp right))
+def c_ifz := c_add.comp <| pair
+  (c_mul.comp <| pair (c_sg'.comp left) (left.comp right))
+  (c_mul.comp <| pair (c_sg.comp left)  (right.comp right))
 @[cp] theorem c_ifz_prim : code_prim c_ifz := by unfold c_ifz; apply_cp
-@[simp] theorem c_ifz_evp {O : ℕ → ℕ} : evalp O c_ifz = fun (cab : ℕ) => if cab.l=0 then cab.r.l else cab.r.r := by
-  simp [c_ifz,evalp];
+@[simp, evp_simps] theorem c_ifz_evp {O : ℕ → ℕ} :
+    evalp O c_ifz = fun (cab : ℕ) => if cab.l=0 then cab.r.l else cab.r.r := by
+  simp only [c_ifz, evp_simps];
   funext xs
   have hsplit : xs.l = 0 ∨ ¬ (xs.l = 0) := by exact Or.symm (ne_or_eq xs.l 0)
   cases hsplit with
   | inl h => simp [h]
   | inr h => simp [h]
-theorem c_ifz_ev' {O : ℕ → ℕ} : eval O c_ifz = fun (cab : ℕ) => if cab.l=0 then cab.r.l else cab.r.r := by rw [← evalp_eq_eval c_ifz_prim]; simp only [c_ifz_evp];
-@[simp] theorem c_ifz_ev {O : ℕ → ℕ} {cab} : eval O c_ifz cab = if cab.l=0 then cab.r.l else cab.r.r := by
+theorem c_ifz_ev' {O : ℕ → ℕ} :
+    eval O c_ifz = fun (cab : ℕ) => if cab.l=0 then cab.r.l else cab.r.r := by
+  rw [← evalp_eq_eval c_ifz_prim]; simp only [c_ifz_evp];
+@[simp] theorem c_ifz_ev {O : ℕ → ℕ} {cab} :
+    eval O c_ifz cab = if cab.l=0 then cab.r.l else cab.r.r := by
   simp [c_ifz_ev']
 end Oracle.Single.Code
 end ifz
@@ -420,15 +477,19 @@ section ift
 namespace Oracle.Single.Code
 def c_ift := c_ifz.comp₂ (c_sg'.comp <| left) right
 @[cp] theorem c_ift_prim : code_prim c_ift := by unfold c_ift; apply_cp
-@[simp] theorem c_ift_evp {O : ℕ → ℕ} : evalp O c_ift = fun (cab : ℕ) => if (n2b cab.l) then cab.r.l else cab.r.r := by
-  simp [c_ift,evalp];
+@[simp, evp_simps] theorem c_ift_evp {O : ℕ → ℕ} :
+    evalp O c_ift = fun (cab : ℕ) => if (n2b cab.l) then cab.r.l else cab.r.r := by
+  simp only [c_ift, evp_simps];
   funext xs
   have hsplit : xs.l = 0 ∨ ¬ (xs.l = 0) := by exact Or.symm (ne_or_eq xs.l 0)
   cases hsplit with
   | inl h => simp [h, n2b]
   | inr h => simp [h, n2b]
-theorem c_ift_ev' {O : ℕ → ℕ} : eval O c_ift = fun (cab : ℕ) => if (n2b cab.l) then cab.r.l else cab.r.r := by rw [← evalp_eq_eval c_ift_prim]; simp only [c_ift_evp];
-@[simp] theorem c_ift_ev {O : ℕ → ℕ} {cab} : eval O c_ift cab = if (n2b cab.l) then cab.r.l else cab.r.r := by
+theorem c_ift_ev' {O : ℕ → ℕ} :
+    eval O c_ift = fun (cab : ℕ) => if (n2b cab.l) then cab.r.l else cab.r.r := by
+  rw [← evalp_eq_eval c_ift_prim]; simp only [c_ift_evp];
+@[simp] theorem c_ift_ev {O : ℕ → ℕ} {cab} :
+    eval O c_ift cab = if (n2b cab.l) then cab.r.l else cab.r.r := by
   simp [c_ift_ev']
 end Oracle.Single.Code
 end ift
@@ -437,19 +498,20 @@ section nat_iterate
 namespace Oracle.Single.Code
 def c_nat_iterate (cf : Code) :=
   prec
-  c_id
-  (cf.comp (right.comp right))
+    c_id
+    (cf.comp (right.comp right))
 
-@[cp] theorem c_nat_iterate_prim {cf} (hcf : code_prim cf) : code_prim (c_nat_iterate cf) := by unfold c_nat_iterate; apply_cp
-@[simp] theorem c_nat_iterate_evp {O : ℕ → ℕ} {cf input i} : evalp O (c_nat_iterate cf) ⟪input, i⟫ = (evalp O cf)^[i] (input) := by
-  simp [c_nat_iterate]
+@[cp] theorem c_nat_iterate_prim {cf} (hcf : code_prim cf) : code_prim (c_nat_iterate cf) := by
+  unfold c_nat_iterate; apply_cp
+@[simp, evp_simps] theorem c_nat_iterate_evp {O : ℕ → ℕ} {cf input i} :
+    evalp O (c_nat_iterate cf) ⟪input, i⟫ = (evalp O cf)^[i] (input) := by
+  simp only [c_nat_iterate, evp_simps]
+  simp only [unpaired, unpair_pair, pair_r]
   induction i with
   | zero => simp
   | succ n ih =>
-    simp [ih]
+    simp only [ih, Function.iterate_succ, Function.comp_apply]
     exact Eq.symm (Function.iterate_succ_apply' (evalp O cf) n input)
--- @[simp] theorem c_nat_iterate_ev :eval O (c_nat_iterate cf) ⟪input, i⟫ = (evalp O cf)^[i] (input) := by
---     simp [← evalp_eq_eval c_nat_iterate_prim]
 end Oracle.Single.Code
 end nat_iterate
 
@@ -457,8 +519,10 @@ section mul2
 namespace Oracle.Single.Code
 def c_mul2 := c_mul.comp₂ c_id (c_const 2)
 @[cp] theorem c_mul2_prim : code_prim c_mul2 := by unfold c_mul2; apply_cp
-@[simp] theorem c_mul2_evp {O : ℕ → ℕ} : evalp O c_mul2 = fun x => x*2 := by simp [c_mul2]
-@[simp] theorem c_mul2_ev {O : ℕ → ℕ} : eval O c_mul2 = (fun x => x*(2 : ℕ)) := by rw [← evalp_eq_eval c_mul2_prim]; simp only [c_mul2_evp];
+@[simp, evp_simps] theorem c_mul2_evp {O : ℕ → ℕ} : evalp O c_mul2 = fun x => x*2 := by
+  simp [c_mul2]
+@[simp, evp_simps] theorem c_mul2_ev {O : ℕ → ℕ} : eval O c_mul2 = (fun x => x*(2 : ℕ)) := by
+  rw [← evalp_eq_eval c_mul2_prim]; simp only [c_mul2_evp];
 end Oracle.Single.Code
 end mul2
 
@@ -466,9 +530,10 @@ section max
 namespace Oracle.Single.Code
 def c_max := c_if_le_te.comp₄ left right right left
 @[cp] theorem c_max_prim : code_prim c_max := by unfold c_max; apply_cp
-@[simp] theorem c_max_evp {O : ℕ → ℕ} : evalp O c_max = unpaired2 Nat.max := by
-  simp [c_max,evalp, -pair_lr]
+@[simp, evp_simps] theorem c_max_evp {O : ℕ → ℕ} : evalp O c_max = unpaired2 Nat.max := by
+  simp only [c_max, evp_simps]
   exact rfl
-@[simp] theorem c_max_ev {O : ℕ → ℕ} : eval O c_max = unpaired2 Nat.max := by rw [← evalp_eq_eval c_max_prim]; simp only [c_max_evp]
+@[simp, evp_simps] theorem c_max_ev {O : ℕ → ℕ} : eval O c_max = unpaired2 Nat.max := by
+  rw [← evalp_eq_eval c_max_prim]; simp only [c_max_evp]
 end Oracle.Single.Code
 end max
